WIP: update fst shadow

proof/invariants/UpdateShadow1StructurePrepare.v
@@ -40,7 +40,229 @@ Invariants StateLib Model.Hardware  Model.MAL
 DependentTypeLemmas Model.Lib InternalLemmas PropagatedProperties UpdateMappedPageContent
 UpdateShadow1Structure.
 Require Import Coq.Logic.ProofIrrelevance Omega List Bool. 
+(*match pt, idx, vaValue with 
+|ptSh1FstVA, idxFstVA, fstVA  =>
+|ptSh1SndVA, idxSndVA, sndVA =>
+|ptSh1TrdVA, idxTrdVA, trdVA => 
+| _, _, _ => True ->*)
+Definition PCToGeneralizePropagatedPropertiesPrepareUpdateShadow1Structure  b1 b2 b3 b4 b5 b6  
+(vaValue fstVA sndVA trdVA:vaddr) (ptMMU ptSh1 pg ptSh1FstVA ptSh1SndVA ptSh1TrdVA phyMMUaddr 
+phySh1addr phySh2addr ptMMUFstVA ptMMUSndVA ptMMUTrdVA :page) 
+(idxFstVA idxSndVA idxTrdVA idx:index):=
+(ptSh1 =ptSh1FstVA /\ idx= idxFstVA /\ vaValue = fstVA /\ pg=phyMMUaddr /\ ptMMU= ptMMUFstVA  /\ b1 = true /\ b4=false /\ b3 = b6 /\ b2 = b5) 
+\/ (ptSh1 =ptSh1SndVA /\ idx= idxSndVA /\ vaValue = sndVA /\ pg=phySh1addr /\ ptMMU= ptMMUSndVA /\ b2 = true /\ b5=false /\ b1= b4 /\ b3 = b6) 
+\/ (ptSh1 = ptSh1TrdVA/\ idx= idxTrdVA /\ vaValue = trdVA /\ pg=phySh2addr /\ ptMMU= ptMMUTrdVA /\ b3 = true /\ b6=false /\ b1=b4 /\ b2=b5).
 
+Lemma propagatedPropertiesPrepareUpdateShadow1Structure b1 b2 b3 b4 b5 b6  (vaValue:vaddr) (ptMMU ptSh1  pg:page) (idx:index) s 
+       ptMMUTrdVA phySh2addr phySh1addr indMMUToPrepare
+       ptMMUFstVA phyMMUaddr lastLLTable phyPDChild currentShadow2 phySh2Child currentPD
+       ptSh1TrdVA ptMMUSndVA ptSh1SndVA ptSh1FstVA currentShadow1 descChildphy phySh1Child
+       currentPart trdVA nextVA vaToPrepare sndVA fstVA nbLgen l idxFstVA idxSndVA idxTrdVA zeroI:
+       
+PCToGeneralizePropagatedPropertiesPrepareUpdateShadow1Structure b1 b2 b3 b4 b5 b6  
+vaValue fstVA sndVA trdVA ptMMU ptSh1 pg ptSh1FstVA ptSh1SndVA ptSh1TrdVA phyMMUaddr phySh1addr phySh2addr
+ ptMMUFstVA ptMMUSndVA ptMMUTrdVA idxFstVA idxSndVA idxTrdVA idx-> 
+propagatedPropertiesPrepare s ptMMUTrdVA phySh2addr phySh1addr indMMUToPrepare
+       ptMMUFstVA phyMMUaddr lastLLTable phyPDChild currentShadow2 phySh2Child currentPD
+       ptSh1TrdVA ptMMUSndVA ptSh1SndVA ptSh1FstVA currentShadow1 descChildphy phySh1Child
+       currentPart trdVA nextVA vaToPrepare sndVA fstVA nbLgen l false false false b1 b2 b3
+        idxFstVA idxSndVA idxTrdVA zeroI -> 
+propagatedPropertiesPrepare  {|  currentPartition := currentPartition s;
+                                 memory := add ptSh1 idx (VE {| pd := false; va := vaValue |}) (memory s) beqPage beqIndex |}
+       ptMMUTrdVA phySh2addr phySh1addr indMMUToPrepare
+       ptMMUFstVA phyMMUaddr lastLLTable phyPDChild currentShadow2 phySh2Child currentPD
+       ptSh1TrdVA ptMMUSndVA ptSh1SndVA ptSh1FstVA currentShadow1 descChildphy phySh1Child
+       currentPart trdVA nextVA vaToPrepare sndVA fstVA nbLgen l false false false b4 b5 b6
+       idxFstVA idxSndVA idxTrdVA zeroI.
+Proof.
+set (s':= {|currentPartition:= _ |}) in *.
+intros Hor Hprops.
+unfold propagatedPropertiesPrepare in *.
+assert((defaultPage =? ptMMU) = false 
+        /\ entryPresentFlag ptMMU (StateLib.getIndexOfAddr vaValue fstLevel) true s
+        (* /\ entryUserFlag ptMMU (StateLib.getIndexOfAddr vaValue fstLevel) true s *)
+        /\ isEntryPage ptMMU (StateLib.getIndexOfAddr vaValue fstLevel) pg s
+        /\ isPE ptMMU idx s
+        /\ getTableAddrRoot ptMMU PDidx (currentPartition s) vaValue s
+        /\ (defaultPage =? ptSh1 ) = false
+        /\ isVE ptSh1 idx s
+        /\ StateLib.getIndexOfAddr vaValue fstLevel = idx
+        /\ beqVAddr defaultVAddr vaValue = false
+        /\ (defaultPage =? ptSh1) = false
+        /\ getTableAddrRoot ptSh1 sh1idx (currentPartition s) vaValue s
+) as (Hnotdef &Hpres (* &Huser *) & Hentryp & Hpe & Htblmmu & Hsh1notdef
+& Hve & Hidx  & Hvanotnull & Hptsh1notnull & Htblsh1).
+{ unfold PCToGeneralizePropagatedPropertiesPrepareUpdateShadow1Structure in *;intuition;subst;trivial. }
+assert(Hlookup :exists entry, 
+ lookup ptSh1 idx (memory s) beqPage beqIndex = Some (VE entry)).
+{ assert(Hva : isVE ptSh1 idx s) by trivial.  
+  unfold isVE in *.
+ subst. 
+ destruct(lookup ptSh1
+          (StateLib.getIndexOfAddr vaValue fstLevel) (memory s)
+          );intros; try now contradict Hva.
+ destruct v; try now contradict Hva.
+ do 2 f_equal.
+ exists v;trivial. }
+ destruct Hlookup as(v0 & Hlookup).
+ 
+assert (Hreadflag : isPartitionFalse ptSh1 idx s ).
+{ admit.  (* unfold isPartitionFalse.
+unfold consistency in *. 
+assert(Haccessva : accessibleVAIsNotPartitionDescriptor s) by intuition.
+unfold accessibleVAIsNotPartitionDescriptor in *.
+assert (Hflag : getPDFlag currentShadow1 vaValue s = false).
+{ eapply Haccessva with (partition:= (currentPartition s)) (pd:= currentPD) (page0:=pg).
+  unfold consistency in *.
+  unfold currentPartitionInPartitionsList in *.
+  intuition.
+  apply nextEntryIsPPgetPd; intuition.
+  apply nextEntryIsPPgetFstShadow;intuition.
+  intuition;subst.  
+  eapply isAccessibleMappedPage2  with (currentPartition s) ptMMU;trivial.
+  intros;subst;split;trivial. }
+apply getPDFlagReadPDflag with currentShadow1 vaValue currentPart;trivial.
+intuition;subst;trivial.
+intros;intuition;subst;trivial. *) }
+assert(Hpartitions: getPartitions multiplexer s' = getPartitions multiplexer s) by 
+(apply getPartitionsAddDerivation with v0;trivial).
+intuition;subst;trivial;simpl.
++ apply kernelDataIsolationUpdtateSh1Structure with (entry:= v0);trivial.
++ apply partitionsIsolationUpdtateSh1Structure with (entry:= v0);trivial.
++ apply verticalSharingUpdtateSh1Structure  with (entry:= v0);trivial.
++ eapply consistencyUpdtateSh1Structure with (level0:= nbLgen) (entry:=v0)
+  (currentPD:=currentPD) (ptVaInCurPartpd:=ptMMU) (phyVaChild:=pg);intuition;unfold consistency in *;
+  intuition.
++ apply getTableRootAddDerivation with  (StateLib.getIndexOfAddr trdVA fstLevel) v0 isPE;trivial;intros;split;
+  subst;trivial.
++ apply isPEAddDerivation with v0;trivial.
++ unfold PCToGeneralizePropagatedPropertiesPrepareUpdateShadow1Structure in *.
+   assert (Hi : exists va : vaddr,
+         isEntryVA ptSh1TrdVA (StateLib.getIndexOfAddr trdVA fstLevel) va s/\ 
+         beqVAddr defaultVAddr va = b3 ) by trivial.
+  destruct Hi as (va & Hva & Hderiv).
+  destruct Hor as [Hor|[Hor|Hor]];
+  intuition;subst.
+  - exists va;split;trivial.
+    apply isEntryVAAddDerivation; trivial.
+    eapply toApplyPageTablesOrIndicesAreDifferent with 
+      trdVA  fstVA (currentPartition s)
+      currentShadow1 sh1idx nbLgen isVE s ;trivial.
+    right;left; trivial.
+    rewrite checkVAddrsEqualityWOOffsetPermut;trivial.
+    intros;split;subst;trivial.
+    intros;split;subst;trivial.
+  - exists va;split;trivial.
+   apply isEntryVAAddDerivation; trivial.
+   eapply toApplyPageTablesOrIndicesAreDifferent with 
+    trdVA  sndVA (currentPartition s)
+    currentShadow1 sh1idx nbLgen isVE s ;trivial.
+   right;left; trivial.
+   rewrite checkVAddrsEqualityWOOffsetPermut;trivial.
+   intros;split;subst;trivial.
+   intros;split;subst;trivial.
+  - exists trdVA;split;trivial.
+    unfold isEntryVA. cbn.
+    assert(Hpairs :  beqPairs (ptSh1TrdVA,  StateLib.getIndexOfAddr trdVA fstLevel)
+      (ptSh1TrdVA,  StateLib.getIndexOfAddr trdVA fstLevel)
+    beqPage beqIndex = true). 
+    apply beqPairsTrue;split;trivial.
+    rewrite Hpairs.
+    simpl;trivial.
++ apply getTableRootAddDerivation with  (StateLib.getIndexOfAddr trdVA fstLevel) v0 isVE;trivial;intros;split;
+  subst;trivial.
++ apply isVEAddDerivation with v0; trivial.
++ apply isEntryPageAddDerivation with v0; trivial.
++ apply entryPresentFlagAddDerivation with v0; trivial.
++ apply entryUserFlagAddDerivation  with v0; trivial.
++ apply getTableRootAddDerivation with  (StateLib.getIndexOfAddr sndVA fstLevel) v0 isPE;trivial; intros;split;
+  subst;trivial.
++ apply isPEAddDerivation  with v0; trivial.
++ unfold PCToGeneralizePropagatedPropertiesPrepareUpdateShadow1Structure in *.
+   assert (Hi : exists va : vaddr,
+         isEntryVA ptSh1SndVA (StateLib.getIndexOfAddr sndVA fstLevel) va s/\ 
+         beqVAddr defaultVAddr va = b2 ) by trivial.
+  destruct Hi as (va & Hva & Hderiv).
+  destruct Hor as [Hor|[Hor|Hor]];
+  intuition;subst.
+  - exists va;split;trivial.
+    apply isEntryVAAddDerivation; trivial.
+    eapply toApplyPageTablesOrIndicesAreDifferent with 
+      sndVA  fstVA (currentPartition s)
+      currentShadow1 sh1idx nbLgen isVE s ;trivial.
+    right;left; trivial.
+    rewrite checkVAddrsEqualityWOOffsetPermut;trivial.
+    intros;split;subst;trivial.
+    intros;split;subst;trivial.
+  - exists sndVA;split;trivial.
+    unfold isEntryVA. cbn.
+    assert(Hpairs :  beqPairs (ptSh1SndVA,  StateLib.getIndexOfAddr sndVA fstLevel)
+      (ptSh1SndVA,  StateLib.getIndexOfAddr sndVA fstLevel)
+    beqPage beqIndex = true). 
+    apply beqPairsTrue;split;trivial.
+    rewrite Hpairs.
+    simpl;trivial.
+  - exists va;split;trivial.
+    apply isEntryVAAddDerivation; trivial.
+    eapply toApplyPageTablesOrIndicesAreDifferent with 
+    sndVA trdVA (currentPartition s)
+    currentShadow1 sh1idx nbLgen isVE s ;trivial.
+    right;left; trivial.
+    intros;split;subst;trivial.
+    intros;split;subst;trivial.
++ apply getTableRootAddDerivation with  (StateLib.getIndexOfAddr sndVA fstLevel) v0 isVE;trivial;intros;split;
+  subst;trivial.
++ apply isVEAddDerivation with v0; trivial.
++ unfold PCToGeneralizePropagatedPropertiesPrepareUpdateShadow1Structure in *.
+   assert (Hi : exists va : vaddr,
+         isEntryVA ptSh1FstVA (StateLib.getIndexOfAddr fstVA fstLevel) va s/\ 
+         beqVAddr defaultVAddr va = b1 ) by trivial.
+  destruct Hi as (va & Hva & Hderiv).
+  destruct Hor as [Hor|[Hor|Hor]];
+  intuition;subst.
+  - exists fstVA;split;trivial.
+    unfold isEntryVA. cbn.
+    assert(Hpairs :  beqPairs (ptSh1FstVA,  StateLib.getIndexOfAddr fstVA fstLevel)
+      (ptSh1FstVA,  StateLib.getIndexOfAddr fstVA fstLevel)
+    beqPage beqIndex = true). 
+    apply beqPairsTrue;split;trivial.
+    rewrite Hpairs.
+    simpl;trivial.  
+  - exists va;split;trivial.
+    apply isEntryVAAddDerivation; trivial.
+    eapply toApplyPageTablesOrIndicesAreDifferent with 
+      fstVA sndVA (currentPartition s)
+      currentShadow1 sh1idx nbLgen isVE s ;trivial.
+    right;left; trivial.
+    intros;split;subst;trivial.
+    intros;split;subst;trivial.    
+  - exists va;split;trivial.
+    apply isEntryVAAddDerivation; trivial.
+    eapply toApplyPageTablesOrIndicesAreDifferent with 
+    fstVA trdVA (currentPartition s)
+    currentShadow1 sh1idx nbLgen isVE s ;trivial.
+    right;left; trivial.
+    intros;split;subst;trivial.
+    intros;split;subst;trivial.
++ apply getTableRootAddDerivation with  (StateLib.getIndexOfAddr fstVA fstLevel) v0 isVE;trivial;intros;split;
+  subst;trivial.
++ apply isVEAddDerivation with v0; trivial.
++ apply isEntryPageAddDerivation with v0; trivial.
++ apply entryPresentFlagAddDerivation with v0; trivial.
++ apply entryUserFlagAddDerivation  with v0; trivial.
++ apply getTableRootAddDerivation with  (StateLib.getIndexOfAddr fstVA fstLevel) v0 isPE;trivial;intros;split;
+  subst;trivial.
++ apply isPEAddDerivation with v0; trivial.
++ apply entryUserFlagAddDerivation  with v0; trivial.
++ apply entryPresentFlagAddDerivation with v0; trivial.
++ apply isEntryPageAddDerivation with v0; trivial.
++ apply isEntryPageAddDerivation with v0; trivial.
++ apply nextEntryIsPPAddDerivation with v0; trivial.
++ apply nextEntryIsPPAddDerivation with v0; trivial.
++ apply nextEntryIsPPAddDerivation with v0; trivial.
++ rewrite Hpartitions;trivial.
+Admitted.
+ 
 Lemma writeVirEntryFstVA ptMMUTrdVA phySh2addr phySh1addr indMMUToPrepare ptMMUFstVA phyMMUaddr lastLLTable phyPDChild
       currentShadow2 phySh2Child currentPD ptSh1TrdVA ptMMUSndVA ptSh1SndVA ptSh1FstVA currentShadow1 descChildphy phySh1Child
       currentPart trdVA nextVA vaToPrepare sndVA fstVA nbLgen l idxFstVA idxSndVA idxTrdVA zeroI lpred:
@@ -69,5 +291,12 @@ Lemma writeVirEntryFstVA ptMMUTrdVA phySh2addr phySh1addr indMMUToPrepare ptMMUF
    /\ isWellFormedMMUTables phyMMUaddr s 
    /\ isWellFormedFstShadow lpred phySh1addr s 
    /\ isWellFormedSndShadow lpred phySh2addr s}}.
-   Proof.
-   Admitted.
+Proof.
+eapply weaken. 
+eapply WP.writeVirEntry.
+simpl;intros.
+intuition.
+apply propagatedPropertiesPrepareUpdateShadow1Structure with true true true ptMMUFstVA phyMMUaddr; trivial.
+unfold PCToGeneralizePropagatedPropertiesPrepareUpdateShadow1Structure.
+left;intuition.
+Admitted.
